src/lib/sparse/Kuiper.Sparse.Matrix.PtsTo.fst
@@ -1,0 +1,747 @@
+module Kuiper.Sparse.Matrix.PtsTo
+
+#lang-pulse
+
+open Kuiper
+open FStar.Tactics.V2 { exact }
+open Kuiper.EMatrix
+open Kuiper.Array.Vectorized
+open Kuiper.Sparse.Common
+open Kuiper.Array2 { array2, layout }
+
+module M = Kuiper.Array2
+module T = Kuiper.Tensor
+open Kuiper.Array2.Strided { strided_row_major }
+
+(* SL props sobre cells *)
+
+let matrix_live_cell
+  (#et : Type0)
+  (#rows #cols : nat)
+  (#lm : M.layout rows cols)
+  (gm : array2 et lm)
+  (i : natlt rows)
+  (j : natlt cols)
+: slprop
+= exists* v. M.pts_to_cell gm (i, j) v
+
+let matrix_pts_to_vec
+  (#et : Type0) {| sized et, has_vec_cpy et |}
+  (#rows #cols : nat)
+  (#l : layout rows cols)
+  (gm : array2 et l)
+  (i : natlt rows)
+  (j : natlt cols { j + chunk et <= cols })
+  (v : lseq et (chunk et))
+: slprop
+= forall+ (k : natlt (chunk et)). M.pts_to_cell gm (i, j + k) (v @! k)
+
+let matrix_live_vec
+  (#et : Type0) {| sized et, has_vec_cpy et |}
+  (#rows #cols : nat)
+  (#l : layout rows cols) {| T.ctlayout l, strided : strided_row_major l |}
+  (gm : array2 et l)
+  (i : natlt rows)
+  (j : natlt cols { j + chunk et <= cols })
+: slprop
+= exists* v. matrix_pts_to_vec gm i j v
+
+let seq_chunk
+  (#et : Type0) {| sized et, has_vec_cpy et |}
+  (#n : nat)
+  (s : lseq et n)
+  (k : nat { k + chunk et <= n })
+: GTot (lseq et (chunk et))
+= Seq.slice s k (k + chunk et)
+
+unfold
+let matrix_pts_to_vec_slice
+  (#et : Type0) {| sized et, has_vec_cpy et |}
+  (#rows #cols : nat)
+  (#l : layout rows cols) {| T.ctlayout l, strided : strided_row_major l |}
+  (gm : array2 et l)
+  (i : natlt rows)
+  (j : natlt cols { j + chunk et <= cols })
+  (#n : nat)
+  (v : lseq et n)
+  (k : nat { k + chunk et <= n })
+: slprop
+// = forall+ (x : natlt (chunk et)). M.pts_to_cell gm (i, j + x) (v @! k + x)
+= matrix_pts_to_vec gm i j (seq_chunk v k)
+
+let matrix_pts_to_cell_in_bounds
+  (#et : Type0)
+  (#rows #cols : nat)
+  (#lm : M.layout rows cols)
+  (gm : array2 et lm)
+  (i : natlt rows)
+  (j : nat)
+  (v : et)
+: slprop
+= when__ (j < cols) (fun _ -> M.pts_to_cell gm (i, j) v)
+
+let matrix_live_cell_in_bounds
+  (#et : Type0)
+  (#rows #cols : nat)
+  (#lm : M.layout rows cols)
+  (gm : array2 et lm)
+  (i : natlt rows)
+  (j : nat)
+: slprop
+= exists* v. matrix_pts_to_cell_in_bounds gm i j v
+
+let matrix_pts_to_vec_in_bounds
+  (#et : Type0) {| sized et, has_vec_cpy et |}
+  (#rows #cols : nat { chunk et /? cols })
+  (#l : layout rows cols)
+  (gm : array2 et l)
+  (i : natlt rows)
+  (j : nat { chunk et /? j })
+  // (v : (squash (j < cols)) -> GTot (lseq et (chunk et)))
+  (v : lseq et (chunk et))
+: slprop
+=
+  when__ (j < cols) (fun _ -> matrix_pts_to_vec gm i j v)
+
+ghost
+fn matrix_pts_to_vec_in_bounds_equiv
+  (#et : Type0) {| sized et, has_vec_cpy et |}
+  (#rows #cols : nat { chunk et /? cols })
+  (#l : layout rows cols) {| T.ctlayout l, strided : strided_row_major l |}
+  (gm : array2 et l)
+  (i : natlt rows)
+  (j : nat { chunk et /? j })
+  (v w : lseq et (chunk et))
+  requires matrix_pts_to_vec_in_bounds gm i j v
+  requires pure (v == w)
+  ensures matrix_pts_to_vec_in_bounds gm i j w
+{
+  unfold matrix_pts_to_vec_in_bounds gm;
+  if (j < cols)
+  {
+    when__elim_true _ _;
+    rewrite each v as w;
+    when__intro_true (j < cols) (matrix_pts_to_vec gm i j w);
+    fold matrix_pts_to_vec_in_bounds gm i j w;
+  }
+  else
+  {
+    when__elim_false _ _;
+    when__intro_false (j < cols) (fun _ -> matrix_pts_to_vec gm i j w);
+    fold matrix_pts_to_vec_in_bounds gm i j w;
+  }
+
+}
+
+
+let matrix_live_vec_in_bounds
+  (#et : Type0) {| sized et, has_vec_cpy et |}
+  (#rows #cols : nat { chunk et /? cols })
+  (#l : layout rows cols)
+  (gm : array2 et l)
+  (i : natlt rows)
+  (j : nat { chunk et /? j })
+: slprop
+= exists* v. matrix_pts_to_vec_in_bounds gm i j v
+
+unfold
+let matrix_pts_to_vec_slice_in_bounds
+  (#et : Type0) {| sized et, has_vec_cpy et |}
+  (#rows #cols : nat { chunk et /? cols })
+  (#l : layout rows cols) {| T.ctlayout l, strided : strided_row_major l |}
+  (gm : array2 et l)
+  (i : natlt rows)
+  (j : nat { chunk et /? j })
+  (#n : nat)
+  (v : lseq et n)
+  (k : nat { k + chunk et <= n })
+: slprop
+= matrix_pts_to_vec_in_bounds gm i j (seq_chunk v k)
+
+(* fold/unfold *)
+
+ghost
+fn fold_matrix_pts_to_vec_in_bounds
+  (#et : Type0) {| sized et, has_vec_cpy et |}
+  (#rows #cols : nat { chunk et /? cols })
+  (#l : layout rows cols) {| T.ctlayout l, strided : strided_row_major l |}
+  (gm : array2 et l)
+  (i : natlt rows)
+  (j : nat { chunk et /? j })
+  (v : lseq et (chunk et))
+  (#_ : squash (j < cols))
+  requires matrix_pts_to_vec gm i j v
+  ensures matrix_pts_to_vec_in_bounds gm i j v
+{
+  when__intro_true (j < cols) (matrix_pts_to_vec gm i j v);
+  fold matrix_pts_to_vec_in_bounds gm i j v;
+}
+
+ghost
+fn fold_matrix_pts_to_vec_slice_in_bounds
+  (#et : Type0) {| sized et, has_vec_cpy et |}
+  (#rows #cols : nat { chunk et /? cols })
+  (#l : layout rows cols) {| T.ctlayout l, strided : strided_row_major l |}
+  (gm : array2 et l)
+  (i : natlt rows)
+  (j : nat { chunk et /? j })
+  (#n : nat)
+  (v : lseq et n)
+  (k : nat { k + chunk et <= n })
+  (#_ : squash (j < cols))
+  requires matrix_pts_to_vec_slice gm i j v k
+  ensures matrix_pts_to_vec_slice_in_bounds gm i j v k
+{
+  fold_matrix_pts_to_vec_in_bounds gm i j (seq_chunk v k)
+}
+
+ghost
+fn fold_matrix_pts_to_vec_not_in_bounds
+  (#et : Type0) {| sized et, has_vec_cpy et |}
+  (#rows #cols : nat { chunk et /? cols })
+  (#l : layout rows cols) {| T.ctlayout l, strided : strided_row_major l |}
+  (gm : array2 et l)
+  (i : natlt rows)
+  (j : nat { chunk et /? j })
+  (v : lseq et (chunk et))
+  requires pure (j >= cols)
+  ensures matrix_pts_to_vec_in_bounds gm i j v
+{
+  when__intro_false (j < cols) (fun _ ->
+    matrix_pts_to_vec gm i j v
+  );
+  fold matrix_pts_to_vec_in_bounds gm i j v;
+}
+
+ghost
+fn fold_matrix_pts_to_vec_slice_not_in_bounds
+  (#et : Type0) {| sized et, has_vec_cpy et |}
+  (#rows #cols : nat { chunk et /? cols })
+  (#l : layout rows cols) {| T.ctlayout l, strided : strided_row_major l |}
+  (gm : array2 et l)
+  (i : natlt rows)
+  (j : nat { chunk et /? j })
+  (#n : nat)
+  (v : lseq et n)
+  (k : nat { k + chunk et <= n })
+  requires pure (j >= cols)
+  ensures matrix_pts_to_vec_slice_in_bounds gm i j v k
+{
+  fold_matrix_pts_to_vec_not_in_bounds gm i j (seq_chunk v k);
+}
+
+ghost
+fn unfold_matrix_pts_to_vec_in_bounds
+  (#et : Type0) {| sized et, has_vec_cpy et |}
+  (#rows #cols : nat { chunk et /? cols })
+  (#l : layout rows cols) {| T.ctlayout l, strided : strided_row_major l |}
+  (gm : array2 et l)
+  (i : natlt rows)
+  (j : nat { chunk et /? j })
+  (v : lseq et (chunk et))
+  (#_ : squash (j < cols))
+  requires matrix_pts_to_vec_in_bounds gm i j v
+  ensures matrix_pts_to_vec gm i j v 
+{
+  unfold matrix_pts_to_vec_in_bounds gm i j v;
+  when__elim_true _ _;
+}
+
+ghost
+fn unfold_matrix_live_vec_in_bounds
+  (#et : Type0) {| sized et, has_vec_cpy et |}
+  (#rows #cols : nat { chunk et /? cols })
+  (#l : layout rows cols) {| T.ctlayout l, strided : strided_row_major l |}
+  (gm : array2 et l)
+  (i : natlt rows)
+  (j : nat { chunk et /? j })
+  (#_ : squash (j < cols))
+  requires matrix_live_vec_in_bounds gm i j
+  ensures matrix_live_vec gm i j
+{
+  unfold matrix_live_vec_in_bounds gm;
+  unfold_matrix_pts_to_vec_in_bounds gm i j _;
+  fold matrix_live_vec gm i j;
+}
+
+ghost
+fn unfold_matrix_pts_to_vec_not_in_bounds
+  (#et : Type0) {| sized et, has_vec_cpy et |}
+  (#rows #cols : nat { chunk et /? cols })
+  (#l : layout rows cols) {| T.ctlayout l, strided : strided_row_major l |}
+  (gm : array2 et l)
+  (i : natlt rows)
+  (j : nat { chunk et /? j })
+  (v : lseq et (chunk et))
+  requires pure (j >= cols)
+  requires matrix_pts_to_vec_in_bounds gm i j v
+{
+  unfold matrix_pts_to_vec_in_bounds gm i j v;
+  when__elim_false _ _;
+}
+
+ghost
+fn unfold_matrix_live_vec_not_in_bounds
+  (#et : Type0) {| sized et, has_vec_cpy et |}
+  (#rows #cols : nat { chunk et /? cols })
+  (#l : layout rows cols) {| T.ctlayout l, strided : strided_row_major l |}
+  (gm : array2 et l)
+  (i : natlt rows)
+  (j : nat { chunk et /? j })
+  requires pure (j >= cols)
+  requires matrix_live_vec_in_bounds gm i j
+{
+  unfold matrix_live_vec_in_bounds gm; 
+  unfold_matrix_pts_to_vec_not_in_bounds gm i j _;
+}
+
+(* thread owns in matrix *)
+
+let offset_chunk
+  (et : Type0) {| sized et, has_vec_cpy et |}
+  (j : nat { chunk et /? j })
+  (k : nat)
+  (nthr : nat)
+: Pure nat (requires true) (ensures divides (chunk et))
+=
+  lemma_divides_product (chunk et) (k * nthr);
+  lemma_divides_sum (chunk et) j (k * nthr * chunk et);
+  j + k * nthr * v (chunk et)
+
+unfold
+let thread_live_vec
+  (#et : Type0) {| sized et, has_vec_cpy et |}
+  (#rows #cols : nat { chunk et /? cols })
+  (#l : layout rows cols)
+  (gm : array2 et l)
+  (i : natlt rows)
+  (j : nat { chunk et /? j })
+  (row_tile : nat)
+  (nthr : nat)
+  (k : natlt (row_tile / chunk et))
+: slprop
+= matrix_live_vec_in_bounds gm i (offset_chunk et j k nthr)
+
+let thread_live_tile_vec
+  (#et : Type0) {| sized et, has_vec_cpy et |}
+  (#rows #cols : nat { chunk et /? cols })
+  (#l : layout rows cols) {| T.ctlayout l, strided : strided_row_major l |}
+  (gm : array2 et l)
+  (i : natlt rows)
+  (j : nat { chunk et /? j })
+  (row_tile : nat)
+  (nthr : nat)
+: slprop
+=
+  forall+ (k : natlt (row_tile / chunk et)).
+    thread_live_vec gm i j row_tile nthr k
+
+unfold
+let thread_pts_to_vec_underspec
+  (#et : Type0) {| sized et, has_vec_cpy et |}
+  (#rows #cols : nat { chunk et /? cols })
+  (#l : layout rows cols) {| T.ctlayout l, strided : strided_row_major l |}
+  (gm : array2 et l)
+  (i : natlt rows)
+  (j : nat { chunk et /? j })
+  (#row_tile : nat { chunk et /? row_tile })
+  (s : lseq et row_tile)
+  (nthr : nat)
+  (k : natlt (row_tile / chunk et))
+: slprop
+=
+    matrix_pts_to_vec_slice_in_bounds gm
+      i (offset_chunk et j k nthr)
+      s (k * chunk et)
+
+let thread_pts_to_tile_vec_underspec
+  (#et : Type0) {| sized et, has_vec_cpy et |}
+  (#rows #cols : nat { chunk et /? cols })
+  (#l : layout rows cols) {| T.ctlayout l, strided : strided_row_major l |}
+  (gm : array2 et l)
+  (i : natlt rows)
+  (j : nat { chunk et /? j })
+  (#row_tile : nat { chunk et /? row_tile })
+  (s : lseq et row_tile)
+  (nthr : nat)
+: slprop
+=
+  forall+ (k : natlt (row_tile / chunk et)).
+    thread_pts_to_vec_underspec gm i j s nthr k
+    // matrix_pts_to_cell_vec_in_bounds' gm
+    //   i (offset_chunk et j k nthr tid)
+    //   s (k * chunk et)
+
+let ematrix_row_chunk_
+  (#et : Type0) {| sized et, has_vec_cpy et |}
+  (#rows #cols : nat)
+  (em : ematrix et rows cols)
+  (i : natlt rows)
+  (j : natlt cols { j + chunk et <= cols })
+: GTot (lseq et (chunk et))
+= Seq.init_ghost (chunk et) (fun k -> macc em i (j + k)) 
+
+let ematrix_row_chunk
+  (#et : Type0) {| sized et, has_vec_cpy et |}
+  // usamos pos y no nat porque garantiza que chunk et <= cols
+  (#rows #cols : pos { chunk et /? cols })
+  (em : ematrix et rows cols)
+  (i : natlt rows)
+  (j : natlt cols { chunk et /? j })
+: GTot (lseq et (chunk et))
+= ematrix_row_chunk_ em i j
+
+// TODO mover de acá
+unfold
+let matrix_pts_to_vec_in_matrix_in_bounds
+  (#et : Type0) {| sized et, has_vec_cpy et |}
+  // usamos pos y no nat porque garantiza que chunk et <= cols
+  (#rows #cols : pos { chunk et /? cols })
+  (#l : layout rows cols) {| T.ctlayout l, strided : strided_row_major l |}
+  (gm : array2 et l)
+  (i : natlt rows)
+  (j : nat { chunk et /? j })
+  (em : ematrix et rows cols)
+: slprop
+=
+  when__ (j < cols) (fun _ ->
+    matrix_pts_to_vec gm i j (ematrix_row_chunk em i j)
+  )
+
+unfold
+let thread_pts_to_vec
+  (#et : Type0) {| sized et, has_vec_cpy et |}
+  (#rows #cols : pos { chunk et /? cols })
+  (#l : layout rows cols) {| T.ctlayout l, strided : strided_row_major l |}
+  (gm : array2 et l)
+  (i : natlt rows)
+  (j : nat { chunk et /? j })
+  (em : ematrix et rows cols)
+  (nthr : nat)
+  (k : nat)
+: slprop
+=
+    matrix_pts_to_vec_in_matrix_in_bounds gm
+      i (offset_chunk et j k nthr) em
+
+
+
+let is_ematrix_tile_at
+  (#et : Type0) {| sized et, has_vec_cpy et |}
+  (#rows #cols : nat { chunk et /? cols })
+  (em : ematrix et rows cols)
+  (i : natlt rows)
+  (j : nat { chunk et /? j })
+  (#row_tile : nat { chunk et /? row_tile }) 
+  (s : lseq et row_tile)
+  (nthr : nat)
+  (k : natlt (row_tile / chunk et))
+: Pure prop
+  (requires offset_chunk et j k nthr < cols)
+  (ensures fun _ -> true)
+= 
+  seq_chunk s (k * chunk et) ==
+  ematrix_row_chunk em i (offset_chunk et j k nthr)
+
+let is_ematrix_tile
+  (#et : Type0) {| sized et, has_vec_cpy et |}
+  (#rows #cols : nat { chunk et /? cols })
+  (em : ematrix et rows cols)
+  (i : natlt rows)
+  (j : nat { chunk et /? j })
+  (#row_tile : nat { chunk et /? row_tile }) 
+  (s : lseq et row_tile)
+  (nthr : nat)
+: prop
+=
+  forall (k : natlt (row_tile / chunk et)).
+    offset_chunk et j k nthr < cols ==>
+      is_ematrix_tile_at em i j s nthr k
+
+ghost
+fn fold_thread_pts_to_vec
+  (#et : Type0) {| sized et, has_vec_cpy et |}
+  (#rows #cols : pos { chunk et /? cols })
+  (#l : layout rows cols) {| T.ctlayout l, strided : strided_row_major l |}
+  (gm : array2 et l)
+  (i : natlt rows)
+  (j : nat { chunk et /? j })
+  (em : ematrix et rows cols)
+  (#row_tile : nat { chunk et /? row_tile })
+  (s : lseq et row_tile)
+  (nthr : nat)
+  (k : natlt (row_tile / chunk et))
+  requires thread_pts_to_vec_underspec gm i j s nthr k
+  requires pure (is_ematrix_tile em i j s nthr)
+  ensures thread_pts_to_vec gm i j em nthr k
+{
+  if (offset_chunk et j k nthr < cols)
+  {
+    assert pure (is_ematrix_tile_at em i j s nthr k);
+    matrix_pts_to_vec_in_bounds_equiv gm
+    i (offset_chunk et j k nthr)
+      (seq_chunk s (k * chunk et))
+      (ematrix_row_chunk em i (offset_chunk et j k nthr));
+    unfold matrix_pts_to_vec_in_bounds gm;
+  }
+  else
+  {
+    unfold matrix_pts_to_vec_in_bounds gm;
+    when__elim_false _ _;
+    when__intro_false (offset_chunk et j k nthr< cols)
+      (fun _ ->
+        matrix_pts_to_vec gm
+          i (offset_chunk et j k nthr)
+          (ematrix_row_chunk em i (offset_chunk et j k nthr))
+      );
+  }
+}
+
+let thread_pts_to_tile_vec
+  (#et : Type0) {| sized et, has_vec_cpy et |}
+  (#rows #cols : pos { chunk et /? cols })
+  (#l : layout rows cols) {| T.ctlayout l, strided : strided_row_major l |}
+  (gm : array2 et l)
+  (i : natlt rows)
+  (j : nat { chunk et /? j })
+  (em : ematrix et rows cols)
+  (row_tile : nat { chunk et /? row_tile })
+  (nthr : nat)
+: slprop
+=
+  forall+ (k : natlt (row_tile / chunk et)).
+    thread_pts_to_vec gm i j em nthr k
+
+
+ghost
+fn fold_thread_pts_to_tile_vec
+  (#et : Type0) {| sized et, has_vec_cpy et |}
+  (#rows #cols : pos { chunk et /? cols })
+  (#l : layout rows cols) {| T.ctlayout l, strided : strided_row_major l |}
+  (gm : array2 et l)
+  (i : natlt rows)
+  (j : nat { chunk et /? j })
+  (#row_tile : nat { chunk et /? row_tile })
+  (s : lseq et row_tile)
+  (em : ematrix et rows cols)
+  (nthr : nat)
+  requires thread_pts_to_tile_vec_underspec gm i j s nthr
+  requires pure (is_ematrix_tile em i j s nthr)
+  ensures thread_pts_to_tile_vec gm i j em row_tile nthr
+{
+  unfold thread_pts_to_tile_vec_underspec gm;
+  forevery_map #(natlt (row_tile / chunk et))
+    (fun k -> thread_pts_to_vec_underspec gm i j s nthr k)
+    (fun k -> thread_pts_to_vec gm i j em nthr k)
+    fn k {
+      fold_thread_pts_to_vec gm i j em s nthr k
+    };
+  fold thread_pts_to_tile_vec gm i j em row_tile nthr;
+}
+
+
+unfold
+let matrix_pts_to_cell_in_matrix_in_bounds
+  (#et : Type0)
+  (#rows #cols : nat)
+  (#l : layout rows cols)
+  (gm : array2 et l)
+  (i : natlt rows)
+  (j : nat)
+  (em : ematrix et rows cols)
+: slprop
+=
+  when__ (j < cols) (fun _ ->
+    M.pts_to_cell gm (i, j) (macc em i j)
+  )
+
+let gpu_pts_to_tile
+  (#et : Type0)
+  (#rows #cols : nat)
+  (#l : layout rows cols)
+  (gm : array2 et l)
+  (i : natlt rows)
+  (j : nat)
+  (em : ematrix et rows cols)
+  (row_tile : nat)
+: slprop
+=
+  forall+ (k : natlt row_tile).
+    matrix_pts_to_cell_in_matrix_in_bounds gm i (j + k) em
+
+ghost
+fn unfold_matrix_pts_to_vec_in_matrix_in_bounds
+  (#et : Type0) {| sized et, has_vec_cpy et |}
+  // usamos pos y no nat porque garantiza que chunk et <= cols
+  (#rows #cols : pos { chunk et /? cols })
+  (#l : layout rows cols) {| T.ctlayout l, strided : strided_row_major l |}
+  (gm : array2 et l)
+  (i : natlt rows)
+  (j : nat { chunk et /? j })
+  (em : ematrix et rows cols)
+  requires matrix_pts_to_vec_in_matrix_in_bounds gm i j em
+  ensures forall+ (x : natlt (chunk et)).
+    matrix_pts_to_cell_in_matrix_in_bounds gm i (j + x) em
+
+{
+  if (j < cols)
+  {
+    when__elim_true _ _;
+    unfold matrix_pts_to_vec gm;
+    forevery_ext #(natlt (chunk et))
+      _
+      (fun x ->
+        matrix_pts_to_cell_in_matrix_in_bounds gm
+          i (j + x) em
+      );
+  }
+  else
+  {
+    when__elim_false _ _;
+    forevery_intro_fill #(natlt (chunk et))
+      (fun x ->
+        matrix_pts_to_cell_in_matrix_in_bounds gm
+          i (j + x) em
+      )
+      fn x {
+        when__intro_false (j + x < cols) (fun _ ->
+          M.pts_to_cell gm (i, j + x) (macc em i (j + x))
+        );
+      };
+  }
+}
+
+let thread_offset
+  (et : Type0) {| sized et, has_vec_cpy et |}
+  (j : nat)
+  (tid : nat)
+: Pure nat (requires chunk et /? j) (ensures fun off -> chunk et /? off)
+=
+  lineal_divides (chunk et) j (chunk et) tid;
+  j + tid * v (chunk et)
+
+#push-options "--split_queries always --z3rlimit 10"
+ghost
+fn thread_pts_to_tile_vec_gather
+  (#et : Type0) {| sized et, has_vec_cpy et |}
+  (#rows #cols : pos { chunk et /? cols })
+  (#l : layout rows cols) {| T.ctlayout l, strided : strided_row_major l |}
+  (gm : array2 et l)
+  (i : natlt rows)
+  (j : natlt cols { chunk et /? j })
+  (em : ematrix et rows cols)
+  (nthr : nat)
+  (trow_tile : nat { chunk et /? trow_tile })
+  requires forall+ (tid : natlt nthr).
+    thread_pts_to_tile_vec gm i (thread_offset et j tid) em trow_tile nthr
+  ensures gpu_pts_to_tile gm i j em (trow_tile * nthr)
+{
+  forevery_commute _;
+  forevery_unfactor' (trow_tile * nthr / chunk et)
+    (trow_tile / chunk et) nthr
+    _;
+  forevery_map #(natlt (trow_tile * nthr / chunk et))
+    (fun x ->
+      thread_pts_to_vec gm i (thread_offset et j (x % nthr)) em nthr (x / nthr)
+    )
+    (fun x ->
+      forall+ (y : natlt (chunk et)).
+        matrix_pts_to_cell_in_matrix_in_bounds gm i (j + (x * chunk et + y)) em
+    )
+    fn x {
+      let lem : squash (
+        offset_chunk et (thread_offset et j (x % nthr)) (x / nthr) nthr ==
+        j + x * chunk et
+      ) = calc (==) {
+        offset_chunk et (thread_offset et j (x % nthr)) (x / nthr) nthr;
+        == {}
+        j + (x % nthr) * chunk et + x / nthr * nthr * chunk et;
+        == {}
+        j + (x % nthr + x / nthr * nthr) * chunk et;
+        == { FStar.Math.Lib.lemma_div_def x nthr }
+        j + x * chunk et;
+      };
+      rewrite each offset_chunk et (thread_offset et j (x % nthr)) (x / nthr) nthr
+      as (j + x * chunk et);
+      
+      unfold_matrix_pts_to_vec_in_matrix_in_bounds gm
+        i (j + x * chunk et) em;
+
+      forevery_ext #(natlt (chunk et))
+        _
+        (fun y ->
+          matrix_pts_to_cell_in_matrix_in_bounds gm
+            i (j + (x * chunk et + y)) em
+        );
+    };
+
+  lemma_divides_product_l (chunk et) trow_tile nthr;
+  forevery_unfactor (trow_tile * nthr)
+    (trow_tile * nthr / chunk et) (chunk et)
+    (fun k ->
+      matrix_pts_to_cell_in_matrix_in_bounds gm i (j + k) em
+    );
+  fold gpu_pts_to_tile gm i j em (trow_tile * nthr);
+}
+#pop-options
+
+ghost
+fn gather_gpu_pts_to_tile_row
+  (#et : Type0)
+  (#rows #cols : nat)
+  (#l : layout rows cols)
+  (gm : array2 et l)
+  (i : natlt rows)
+  (em : ematrix et rows cols)
+  (row_tile : pos)
+  requires forall+ (b : natlt (cols `divup` row_tile)).
+    gpu_pts_to_tile gm i (b * row_tile) em row_tile
+  ensures forall+ (j : natlt cols).
+    M.pts_to_cell gm (i, j) (macc em i j)
+{
+  forevery_map #(natlt (cols `divup` row_tile))
+    (fun b ->
+      gpu_pts_to_tile gm i (b * row_tile) em row_tile
+    )
+    (fun b ->
+      forall+ (k : natlt row_tile {b * row_tile + k < cols }).
+        M.pts_to_cell gm (i, b * row_tile + k) (macc em i (b * row_tile + k))
+    )
+    fn b {
+      unfold gpu_pts_to_tile gm;
+      forevery_refine_pred' #(natlt row_tile) (fun k -> b * row_tile + k < cols)
+        _;
+    };
+  forevery_unfactor_ cols row_tile
+    (fun j ->
+      M.pts_to_cell gm (i, j) (macc em i j)
+    );
+}
+
+ghost
+fn gather_gpu_pts_to_tile
+  (#et : Type0)
+  (#rows #cols : nat)
+  (#l : layout rows cols)
+  (gm : array2 et l)
+  (em : ematrix et rows cols)
+  (row_tile : pos)
+  requires pure (fits (M.layout_size l))
+  requires forall+ (r : natlt rows) (b : natlt (cols `divup` row_tile)).
+    gpu_pts_to_tile gm r (b * row_tile) em row_tile
+  ensures gm |-> em
+{
+  forevery_map #(natlt rows)
+    (fun r ->
+      forall+ (b : natlt (cols `divup` row_tile)).
+        gpu_pts_to_tile gm r (b * row_tile) em row_tile 
+    )
+    (fun r ->
+      forall+ (j : natlt cols).
+        M.pts_to_cell gm (r, j) (macc em r j)
+    )
+    fn r {
+      gather_gpu_pts_to_tile_row gm r em row_tile
+    };
+  M.iraise gm;
+}
