src/lib/sparse/Kuiper.Sparse.SPMM.LoadDense.fst
@@ -1,0 +1,467 @@
+module Kuiper.Sparse.SPMM.LoadDense
+
+#lang-pulse
+
+open Kuiper
+open Kuiper.Sparse
+open Kuiper.Sparse.Load
+open Kuiper.Array.Vectorized
+open Kuiper.Array2.Vectorized
+open Kuiper.EMatrix
+open Kuiper.Seq.Common { seq_blit, seq_replace }
+module T = Kuiper.Tensor.Layout
+module M = Kuiper.Array2
+module A = Kuiper.Array1
+
+
+let rec seq_tile_cpy
+  (#et : Type0) {| sized et, has_vec_cpy et |}
+  (#n1 : nat { chunk et /? n1 })
+  (s1 : lseq et n1)
+  (#n2 : nat { chunk et /? n2 })
+  (s2 : lseq et n2)
+  (j2 : nat { chunk et /? j2 })
+  (step : nat)
+  (to : natle (n1 / chunk et))
+: GTot (lseq et n1) (decreases to)
+=
+  if to = 0 then s1 else (
+    lemma_divides_product (chunk et) (to - 1);
+    lemma_divides_product (chunk et) ((to - 1) * step);
+    lemma_divides_sum (chunk et) j2 ((to - 1) * step * chunk et);
+    (seq_blit'
+      (seq_tile_cpy s1 s2 j2 step (to - 1))
+      ((to - 1) * chunk et)
+      s2
+      (j2 + (to - 1) * step * chunk et)
+      (chunk et))
+  )
+
+let lemma_fits_tile_offset
+  (et:Type0) {| sized et, has_vec_cpy et |}
+  (n : nat)
+  (j : nat)
+  (k : natlt (n / chunk et))
+  (step : nat)
+: Lemma
+  (requires fits (j + n * step))
+  (ensures fits (j + k * step * chunk et))
+= ()
+
+let lemma_divides_tile_offset
+  (et:Type0) {| sized et, has_vec_cpy et |}
+  (j k step : sz { fits (j + k * step * chunk et) })
+: Lemma
+  (requires chunk et /? j)
+  (ensures chunk et /? (j +^ k *^ step *^ chunk et))
+=
+  lemma_divides_product (chunk et) (k * step);
+  lemma_divides_sum (chunk et) j (k * step * chunk et)
+
+inline_for_extraction noextract
+fn tile_vec_cpy
+  (#et:Type0) {| sized et, has_vec_cpy et |}
+  (#n1 : sz { chunk et /? n1})
+  (#l1 : A.layout n1) {| T.ctlayout l1, cl1 : cont_layout l1 |}
+  (x1 : A.array1 et l1)
+  (#s1 : erased (lseq et n1))
+  (#n2 : sz { chunk et /? n2})
+  (#l2 : A.layout n2) {| T.ctlayout l2, cl2 : cont_layout l2 |}
+  (x2 : A.array1 et l2)
+  (#f : perm)
+  (#s2 : erased (lseq et n2))
+  (j : sz { chunk et /? j })
+  (step : szp)
+  preserves gpu
+  requires  x1 |-> s1
+  requires  pure (aligned 16 (A.core x1))
+  requires  pure (aligned_cont_layout (chunk et) cl1)
+  preserves x2 |-> Frac f s2
+  requires  pure (aligned 16 (A.core x2))
+  requires  pure (fits (j + n1 * step))
+  requires  pure (aligned_cont_layout (chunk et) cl2)
+  ensures   x1 |-> seq_tile_cpy s1 s2 j step (n1 / chunk et)
+{
+  let mut k : sz = 0sz;
+
+  while (!k <^ n1 /^ chunk et)
+    invariant exists* (vk : szle (n1 / chunk et)).
+      k  |-> (vk <: sz) **
+      x1 |-> seq_tile_cpy s1 s2 j step vk
+  {
+    lemma_fits_tile_offset et n1 j !k step;
+    lemma_divides_tile_offset et j !k step;
+    assert pure (fits (j + !k * step * chunk et));
+    array_vec_cpy_device x1 (!k *^ chunk et) x2 (j +^ !k *^ step *^ chunk et);
+    k := !k +^ 1sz;
+  }
+}
+
+
+let ematrix_tile_cpy
+  (#et : Type0) {| sized et, has_vec_cpy et |}
+  (#m1 #n1 : nat { chunk et /? n1 })
+  (em1 : ematrix et m1 n1)
+  (#m2 #n2 : nat {  chunk et /? n2 })
+  (em2 : ematrix et m2 n2)
+  (row_ind : lseq nat m1 { in_bounds 0 m2 row_ind })
+  (j : nat { chunk et /? j })
+  (step : nat) // tratemos de no usar tid
+: GTot (ematrix et m1 n1)
+= ematrix_from_rows fun i ->
+    seq_tile_cpy
+      (ematrix_row em1 i) (ematrix_row em2 (row_ind @! i))
+      j step (n1 / chunk et)
+
+
+open Kuiper.Array2.Strided { strided_row_major, aligned_strided_row_major }
+
+#push-options "--split_queries always"
+inline_for_extraction noextract
+fn matrix_tile_vec_cpy
+  (#et:Type0) {| sized et, has_vec_cpy et |}
+  (#m1 #n1 : szp { chunk et /? n1 })
+  (#l1 : M.layout m1 n1) {| T.ctlayout l1, srm1 : strided_row_major l1 |}
+  (a1 : M.array2 et l1)
+  (#em1 : ematrix et m1 n1)
+  (#m2 #n2 : szp { chunk et /? n2 })
+  (#l2 : M.layout m2 n2) {| T.ctlayout l2, srm2 : strided_row_major l2 |}
+  (a2 : M.array2 et l2)
+  (#f : perm)
+  (#em2 : ematrix et m2 n2)
+  (j : sz { chunk et /? j })
+  (step : szp)
+  (#lr : A.layout m1) {| T.ctlayout lr |}
+  (row_ind : A.array1 sz lr)
+  (#fr : perm)
+  (#vrow_ind : lseq sz m1)
+  (#_: squash (in_bounds 0 m2 (cast_pos vrow_ind)))
+  preserves gpu
+  requires  a1 |-> em1
+  requires  pure (aligned 16 (M.core a1) /\ aligned_strided_row_major (chunk et) srm1)
+  preserves a2 |-> Frac f em2
+  requires  pure (aligned 16 (M.core a2) /\ aligned_strided_row_major (chunk et) srm2)
+  requires  pure (fits (j + n1 * step))
+  preserves row_ind |-> Frac fr vrow_ind
+  ensures   a1 |-> ematrix_tile_cpy em1 em2 (cast_pos vrow_ind) j step
+{
+  let mut k : sz = 0sz;
+
+  while (!k <^ m1)
+    invariant exists* vk em.
+      k  |-> vk **
+      a1 |-> em **
+      pure (
+        vk <= m1 /\
+        (forall (i : natlt m1 { i < vk }).
+          ematrix_row em i ==
+          seq_tile_cpy
+            (ematrix_row em1 i)
+            (ematrix_row em2 (vrow_ind @! i))
+            j step (n1 / chunk et)
+        ) /\
+        forall (i : natlt m1 { vk <= i }).
+          ematrix_row em i == ematrix_row em1 i
+      )
+  {
+    with em. assert a1 |-> em;
+
+    M.extract_row a1 !k;
+    let ri = A.read row_ind !k;
+    M.extract_row_ro a2 ri; 
+    
+    row_core_lemma a1 !k;
+    aligned_cont_strided_row_major l1 (chunk et) !k;
+    row_core_lemma a2 ri;
+    aligned_cont_strided_row_major l2 (chunk et) ri;
+
+    tile_vec_cpy
+      #_ #_ #_ #_ #_
+      #(Kuiper.Tensor.ctlayout_slice _ 0sz !k) // should not be needed
+      (M.row a1 (v !k))
+      #_ #_ #_
+      #(Kuiper.Tensor.ctlayout_slice _ 0sz ri) // should not be needed
+      (M.row a2 (v ri)) j step;
+    
+    M.restore_row a2 ri;
+    Pulse.Lib.Forall.elim_forall 
+      (seq_tile_cpy
+        (ematrix_row em1 !k) (ematrix_row em2 ri)
+        j step (n1 / chunk et));
+    Pulse.Lib.Trade.elim_trade _ _;
+    
+
+    ematrix_upd_row_lemma em !k 
+      (seq_tile_cpy
+        (ematrix_row em1 !k) (ematrix_row em2 ri)
+        j step (n1 / chunk et));
+    
+    k := !k +^ 1sz;
+  };
+
+  with em. assert a1 |-> em;
+  assert pure (
+    ematrix_rows_equal em (ematrix_tile_cpy em1 em2 (cast_pos vrow_ind) j step)
+  );
+}
+
+let lem1
+  (d : pos) (a b : nat)
+: Lemma
+  (requires b * d <= a /\ a < (b + 1) * d)
+  (ensures a / d = b)
+= ()
+
+let lem2
+  (d : pos) (a b : nat) (c : pos)
+: Lemma
+  (requires a < b * d)
+  (ensures a / d * c * d + a % d < b * c * d)
+= ()
+
+let seq_blit_lemma1
+  (#a:Type)
+  (#n1 : nat)
+  (s1 : lseq a n1) (off1 : natlt n1)
+  (#n2 : nat)
+  (s2 : lseq a n2) (off2 : nat)
+  (cnt : nat { cnt /? n1 /\ cnt /? off1 /\ cnt /? n2 /\ cnt /? off2 } )
+  (k : natlt n1)
+: Lemma
+  (requires k < off1 \/ k >= off1 + cnt)
+  (ensures seq_blit' s1 off1 s2 off2 cnt @! k == s1 @! k)
+=
+  lemma_divides_leq cnt n1 off1;
+  lemma_divides_leq cnt n2 off2
+
+#push-options "--split_queries always"
+let seq_blit_lemma2
+  (#a:Type)
+  (#n1 : nat)
+  (s1 : lseq a n1) (off1 : natlt n1)
+  (#n2 : nat)
+  (s2 : lseq a n2) (off2 : nat)
+  (cnt : nat { cnt /? n1 /\ cnt /? off1 /\ cnt /? n2 /\ cnt /? off2 } )
+  (k : natlt n1)
+: Lemma
+  (requires off1 <= k /\ k < off1 + cnt /\ off2 < n2)
+  (ensures
+    seq_blit' s1 off1 s2 off2 cnt @! k == s2 @! off2 + k - off1
+  )
+=
+  lemma_divides_leq cnt n1 off1;
+  lemma_divides_leq cnt n2 off2;
+  ()
+
+let rec seq_tile_cpy_col_lemma1
+  (#et : Type0) {| sized et, has_vec_cpy et |}
+  (#n1 : nat { chunk et /? n1 })
+  (s1 : lseq et n1)
+  (#n2 : nat { chunk et /? n2 })
+  (s2 : lseq et n2)
+  (j2 : nat { chunk et /? j2 })
+  (step : pos)
+  (to : natle (n1 / chunk et))
+  (k : natlt n1 { k < to * chunk et })
+: Lemma
+  (requires j2 + k / chunk et * step * chunk et + k % chunk et < n2)
+  (ensures
+    seq_tile_cpy s1 s2 j2 step to @! k ==
+    s2 @! j2 + k / chunk et * step * chunk et + k % chunk et
+  )
+= 
+  lemma_divides_product (chunk et) (to - 1);
+  lemma_divides_product (chunk et) ((to - 1) * step);
+  lemma_divides_sum (chunk et) j2 ((to - 1) * step * chunk et);
+  let k1 = j2 + k / chunk et * step * chunk et in
+  let k2 = k % chunk et in
+  if k >= (to - 1) * chunk et
+    then (
+      lem1 (chunk et) k (to - 1);
+      assert k1 = j2 + (to - 1) * step * chunk et;
+      assert k2 = k - (to - 1) * chunk et;
+
+      lem2 (chunk et) k to step;
+      assert k1 + k2 < j2 + to * step * chunk et;
+
+      seq_blit_lemma2
+        (seq_tile_cpy s1 s2 j2 step (to -1))
+        ((to - 1) * chunk et)
+        s2
+        (j2 + (to - 1) * step * chunk et)
+        (chunk et) k
+    )
+    else (
+      lem2 (chunk et) k (to - 1) step;
+      assert k1 + k2 < j2 + (to - 1) * step * chunk et;
+
+      seq_tile_cpy_col_lemma1 s1 s2 j2 step (to - 1) k;
+      seq_blit_lemma1
+        (seq_tile_cpy s1 s2 j2 step (to -1))
+        ((to - 1) * chunk et)
+        s2
+        (j2 + (to - 1) * step * chunk et)
+        (chunk et) k
+    )
+#pop-options
+
+let rec seq_tile_cpy_col_lemma2
+  (#et : Type0) {| sized et, has_vec_cpy et |}
+  (#n1 : nat { chunk et /? n1 })
+  (s1 : lseq et n1)
+  (#n2 : nat { chunk et /? n2 })
+  (s2 : lseq et n2)
+  (j2 : nat { chunk et /? j2 })
+  (step : pos)
+  (to : natle (n1 / chunk et))
+  (k : natlt n1)
+: Lemma
+  (requires j2 + k / chunk et * step * chunk et >= n2)
+  (ensures seq_tile_cpy s1 s2 j2 step to @! k == s1 @! k)
+= 
+  if to = 0 then () else (
+    seq_tile_cpy_col_lemma2 s1 s2 j2 step (to - 1) k;
+
+    lemma_divides_product (chunk et) (to - 1);
+    lemma_divides_product (chunk et) ((to - 1) * step);
+    lemma_divides_sum (chunk et) j2 ((to - 1) * step * chunk et);
+    let k1 = j2 + k / chunk et * step * chunk et in
+    let k2 = k % chunk et in
+
+    if (to - 1) * chunk et <= k && k < to * chunk et then (
+      lem1 (chunk et) k (to - 1);
+      assert k1 = j2 + (to - 1) * step * chunk et;
+      assert k2 = k - (to - 1) * chunk et
+    )
+    else
+      seq_blit_lemma1
+        (seq_tile_cpy s1 s2 j2 step (to - 1))
+        ((to - 1) * chunk et)
+        s2
+        (j2 + (to - 1) * step * chunk et)
+        (chunk et) k
+  )
+
+let ematrix_tile_col
+  (#et : Type0) {| sized et, has_vec_cpy et |}
+  (#m1 #n1 : nat { chunk et /? n1 })
+  (em1 : ematrix et m1 n1)
+  (#m2 #n2 : nat {  chunk et /? n2 })
+  (em2 : ematrix et m2 n2)
+  (row_ind : lseq nat m1 { in_bounds 0 m2 row_ind })
+  (j : nat { chunk et /? j })
+  (step : nat)
+  (k1 : natlt n1)
+: GTot (lseq et m1)
+=
+  let k2 = j + k1 / chunk et * step * chunk et + k1 % chunk et in
+  if k2 < n2 
+    then seq_make_sparse row_ind (ematrix_col em2 k2)
+    else ematrix_col em1 k1
+
+
+let ematrix_tile_col_lemma_
+  (#et : Type0) {| sized et, has_vec_cpy et |}
+  (#m1 #n1 : nat { chunk et /? n1 })
+  (em1 : ematrix et m1 n1)
+  (#m2 #n2 : nat {  chunk et /? n2 })
+  (em2 : ematrix et m2 n2)
+  (row_ind : lseq nat m1 { in_bounds 0 m2 row_ind })
+  (j : nat { chunk et /? j })
+  (step : pos)
+  (k1 : natlt n1)
+: Lemma
+  (requires true)
+  (ensures
+    ematrix_col (ematrix_tile_cpy em1 em2 row_ind j step) k1 ==
+    ematrix_tile_col em1 em2 row_ind j step k1
+  )
+=
+  let c1 = ematrix_col (ematrix_tile_cpy em1 em2 row_ind j step) k1 in
+  let c2 = ematrix_tile_col em1 em2 row_ind j step k1 in
+  let k2 = j + k1 / chunk et * step * chunk et + k1 % chunk et in
+
+  introduce forall i.
+    ematrix_col (ematrix_tile_cpy em1 em2 row_ind j step) k1 @! i==
+    ematrix_tile_col em1 em2 row_ind j step k1 @! i
+  with (
+    if k2 < n2
+      then (
+        seq_tile_cpy_col_lemma1
+          (ematrix_row em1 i)
+          (ematrix_row em2 (row_ind @! i))
+          j
+          step
+          (n1 / chunk et)
+          k1
+      )
+      else (
+        seq_tile_cpy_col_lemma2
+          (ematrix_row em1 i)
+          (ematrix_row em2 (row_ind @! i))
+          j
+          step
+          (n1 / chunk et)
+          k1
+      )
+  );
+  assert Seq.equal
+    (ematrix_col (ematrix_tile_cpy em1 em2 row_ind j step) k1)
+    (ematrix_tile_col em1 em2 row_ind j step k1)
+
+let ematrix_tile_col_lemma
+  (#et : Type0) {| sized et, has_vec_cpy et |}
+  (#m1 #n1 : nat { chunk et /? n1 })
+  (em1 : ematrix et m1 n1)
+  (#m2 #n2 : nat {  chunk et /? n2 })
+  (em2 : ematrix et m2 n2)
+  (row_ind : lseq nat m1 { in_bounds 0 m2 row_ind })
+  (j : nat { chunk et /? j })
+  (step : pos)
+: Lemma
+  (requires true)
+  (ensures
+    ematrix_tile_cpy em1 em2 row_ind j step ==
+    ematrix_from_cols (ematrix_tile_col em1 em2 row_ind j step)
+  )
+=
+  introduce forall k.
+    ematrix_col (ematrix_tile_cpy em1 em2 row_ind j step) k ==
+    ematrix_tile_col em1 em2 row_ind j step k
+  with ematrix_tile_col_lemma_ em1 em2 row_ind j step k;
+  assert ematrix_cols_equal 
+    (ematrix_tile_cpy em1 em2 row_ind j step)
+    (ematrix_from_cols (ematrix_tile_col em1 em2 row_ind j step))
+
+inline_for_extraction noextract
+fn load_dense_matrix
+  (#et:Type0) {| sized et, has_vec_cpy et |}
+  (#m1 #n1 : szp { chunk et /? n1 })
+  (l1 : M.layout m1 n1) {| T.ctlayout l1, srm1 : strided_row_major l1 |}
+  (a1 : M.array2 et l1)
+  (em1 : ematrix et m1 n1)
+  (#m2 #n2 : szp { chunk et /? n2 })
+  (l2 : M.layout m2 n2) {| T.ctlayout l2, srm2 : strided_row_major l2 |}
+  (a2 : M.array2 et l2)
+  (#f : perm)
+  (em2 : ematrix et m2 n2)
+  (j : sz { chunk et /? j })
+  (step : szp)
+  (#lr : A.layout m1) {| T.ctlayout lr |}
+  (row_ind : A.array1 sz lr)
+  (#fr : perm)
+  (vrow_ind : lseq sz m1)
+  (#_: squash (in_bounds 0 m2 (cast_pos vrow_ind)))
+  preserves gpu
+  requires  a1 |-> em1
+  requires  pure (aligned 16 (M.core a1) /\ aligned_strided_row_major (chunk et) srm1)
+  preserves a2 |-> Frac f em2
+  requires  pure (aligned 16 (M.core a2) /\ aligned_strided_row_major (chunk et) srm2)
+  requires  pure (fits (j + n1 * step))
+  preserves row_ind |-> Frac fr vrow_ind
+  ensures   a1 |-> ematrix_from_cols (ematrix_tile_col em1 em2 (cast_pos vrow_ind) j step)
+{
+  matrix_tile_vec_cpy a1 a2 j step row_ind;
+  ematrix_tile_col_lemma em1 em2 (cast_pos vrow_ind) j step;
+  assert a1 |-> ematrix_from_cols (ematrix_tile_col em1 em2 (cast_pos vrow_ind) j step);
+}
