src/lib/sparse/Kuiper.Sparse.SPMM.LoadSparse.fst
@@ -1,0 +1,133 @@
+module Kuiper.Sparse.SPMM.LoadSparse
+
+#lang-pulse
+
+open Kuiper
+open Kuiper.Sparse
+open Kuiper.Sparse.Load
+open Kuiper.Array.Vectorized
+open Kuiper.Array2.Vectorized
+open Kuiper.EMatrix
+
+#push-options "--z3rlimit 10"
+inline_for_extraction noextract
+fn load_array_vec
+  (#et : Type0) {| sized et, has_vec_cpy et |}
+  (#n : sz)
+  (x : gpu_array et n)
+  (#_ : squash (aligned 16 x))
+  (#m : sz)
+  (y : gpu_array et m)
+  (#f : perm)
+  (#s : erased (lseq et m))
+  (i : szle m)
+  (#_ : squash (aligned' 16 y i))
+  (nthr : sz)
+  (tid : szlt nthr)
+  (#_ : squash (nthr * chunk et /? n))
+  (#_ : squash (i + n <= m))
+  preserves gpu ** y |-> Frac f s
+  requires thread_live_chunks x nthr tid
+  ensures thread_pts_to_chunks x s i nthr tid
+{
+  unfold thread_live_chunks x nthr tid;
+
+  forevery_rw_size (n / (nthr * (chunk et))) (n /^ nthr /^ chunk et);
+
+  foreach (n /^ nthr /^ chunk et)
+  (fun k -> gpu_live_vec x ((k * nthr + tid) * chunk et))
+  (fun k ->
+    gpu_pts_to_vec' x ((k * nthr + tid) * chunk et)
+      s (i + (k * nthr + tid) * chunk et)
+  )
+  #(gpu ** y |-> Frac f s)
+  fn k {
+    gpu_array_vec_cpy
+      x ((k *^ nthr +^ tid) *^ chunk et)
+      y (i +^ ((k *^ nthr +^ tid) *^ chunk et));
+  };
+
+  forevery_rw_size (n /^ nthr /^ chunk et) (n / (nthr * (chunk et)));
+
+  fold thread_pts_to_chunks x s i nthr tid;
+}
+#pop-options
+
+// TODO podria generalizar y tomar from y to, aunque cuando
+// repartimos por threads es medio raro
+// Quizas cambiar la def de thread_pts_to
+
+
+inline_for_extraction noextract
+fn load2_array
+  (#et1 #et2 : Type0)
+  (#dsz : sz)
+  (dst1 : gpu_array et1 dsz)
+  (dst2 : gpu_array et2 dsz)
+  (to : szle dsz)
+  (#ssz : sz)
+  (src1 : gpu_array et1 ssz)
+  (src2 : gpu_array et2 ssz)
+  (#f : perm)
+  (#s1 : erased (lseq et1 ssz))
+  (#s2 : erased (lseq et2 ssz))
+  (i : szle ssz)
+  (nthr : sz)
+  (tid : szlt nthr)
+  (#_ : squash (i + to <= ssz))
+  preserves gpu ** src1 |-> Frac f s1 ** src2 |-> Frac f s2
+  requires thread_slice_live dst1 0 to nthr tid
+  requires thread_slice_live dst2 0 to nthr tid
+  requires pure (fits (dsz + nthr))
+  ensures thread_slice_pts_to dst1 0 to s1 i nthr tid
+  ensures thread_slice_pts_to dst2 0 to s2 i nthr tid
+{
+  unfold thread_slice_live dst1 0 to nthr tid;
+  unfold thread_slice_live dst2 0 to nthr tid;
+
+  forevery_zip #(natlt ((to - 0 - tid) `divup` nthr))
+    (fun k -> array_live_cell dst1 (0 + k * nthr + tid))
+    _;
+  forevery_rw_size
+    ((to - 0 - tid) `divup` nthr)
+    ((to +^ (nthr -^ 1sz) -^ tid) /^ nthr);
+
+  foreach ((to +^ (nthr -^ 1sz) -^ tid) /^ nthr)
+    (fun k ->
+      array_live_cell dst1 (0 + k * nthr + tid) **
+      array_live_cell dst2 (0 + k * nthr + tid)
+    )
+    (fun k -> 
+      gpu_pts_to_cell dst1 (k * nthr + tid) (s1 @! i + k * nthr + tid) **
+      gpu_pts_to_cell dst2 (k * nthr + tid) (s2 @! i + k * nthr + tid)
+    )
+    #(gpu ** src1 |-> Frac f s1 ** src2 |-> Frac f s2)
+    fn k {
+      rewrite each (0 + k * nthr + tid) as (k * nthr + tid);
+      gpu_load_cell dst1 (k *^ nthr +^ tid) src1 (i +^ k *^ nthr +^ tid);
+      gpu_load_cell dst2 (k *^ nthr +^ tid) src2 (i +^ k *^ nthr +^ tid);
+    };
+
+  forevery_rw_size
+    ((to +^ (nthr -^ 1sz) -^ tid) /^ nthr)
+    ((to - 0 - tid) `divup` nthr);
+  forevery_unzip _ _;
+
+  forevery_ext #(natlt ((to - 0 - tid) `divup` nthr))
+    (fun x ->
+      gpu_pts_to_cell dst1 (x * nthr + tid) (s1 @! i + x * nthr + tid)
+    )
+    (fun x ->
+      gpu_pts_to_cell dst1 (0 + x * nthr + tid) (s1 @! i + x * nthr + tid)
+    );
+  fold thread_slice_pts_to dst1 0 to s1 i nthr tid;
+
+  forevery_ext #(natlt ((to - 0 - tid) `divup` nthr))
+    (fun x ->
+      gpu_pts_to_cell dst2 (x * nthr + tid) (s2 @! i + x * nthr + tid)
+    )
+    (fun x ->
+      gpu_pts_to_cell dst2 (0 + x * nthr + tid) (s2 @! i + x * nthr + tid)
+    );
+  fold thread_slice_pts_to dst2 0 to s2 i nthr tid;
+}
