src/lib/sparse/Kuiper.Sparse.SPMM.Mask.fst
@@ -1,0 +1,70 @@
+module Kuiper.Sparse.SPMM.Mask
+
+#lang-pulse
+
+open Kuiper
+open Kuiper.Sparse
+open Kuiper.Array.Vectorized
+open Kuiper.Array2.Vectorized
+open Kuiper.EMatrix
+
+inline_for_extraction noextract
+fn gpu_mask_cell
+  (#et : Type0)
+  (#n : sz)
+  (x : gpu_array et n)
+  (i : szlt n)
+  (z : et)
+  preserves gpu
+  requires array_live_cell x i
+  ensures  gpu_pts_to_cell x i z
+{
+  unfold array_live_cell x;
+  gpu_array_write x i z;
+  with s. assert gpu_pts_to_slice x i (i + 1) s;
+  assert pure (Seq.equal s seq![z]);
+}
+
+// TODO podria generalizar y tomar from y to, aunque cuando
+// repartimos por threads es medio raro
+// Quizas cambiar la def de thread_pts_to
+
+inline_for_extraction noextract
+fn mask_array
+  (#et : Type0)
+  (#n : sz)
+  (x : gpu_array et n)
+  (to : szle n)
+  (z : et)
+  (nthr : sz)
+  (tid : szlt nthr)
+  preserves gpu
+  requires thread_slice_live x 0 to nthr tid
+  requires pure (fits (n + nthr))
+  ensures thread_slice_pts_to_value x 0 to z nthr tid
+{
+  unfold thread_slice_live x 0 to nthr tid;
+
+  let to_ : sz = (to +^ (nthr -^ 1sz) -^ tid) /^ nthr;
+  forevery_rw_size ((to - 0 - tid) `divup` nthr) to_;
+
+  foreach to_
+    (fun k ->
+      array_live_cell x (0 + k * nthr + tid)
+    )
+    (fun k ->
+      gpu_pts_to_cell x (k * nthr + tid) z
+    )
+    #gpu
+    fn k {
+      rewrite each (0 + k * nthr + tid) as (k * nthr + tid);
+      gpu_mask_cell x (k *^ nthr +^ tid) z;
+    };
+
+  forevery_rw_size to_ ((to - 0 - tid) `divup` nthr);
+
+  forevery_ext #(natlt ((to - 0 - tid) `divup` nthr))
+    (fun k -> gpu_pts_to_cell x (k * nthr + tid) z)
+    (fun k -> gpu_pts_to_cell x (0 + k * nthr + tid) z);
+  fold thread_slice_pts_to_value x 0 to z nthr tid;
+}
