src/lib/sparse/Kuiper.Sparse.fst
@@ -5,4 +5,7 @@ include Kuiper.Sparse.Common
 include Kuiper.Sparse.Array
 // include Kuiper.Sparse.Array.Iterator
 include Kuiper.Sparse.Matrix
-include Kuiper.Sparse.PtsTo
+// TODO tal vez no esta bueno incluir estos dos porque puede haber coincidencias de nombres
+// se pueden incluir qualified?
+include Kuiper.Sparse.Array.PtsTo
+include Kuiper.Sparse.Matrix.PtsTo
